@@ -231,6 +231,7 @@ import Xv6.KilledDefs
 import Xv6.SpecGrowproc
 import Xv6.UMemLemmas
 import Xv6.UMemWindow
+import Xv6.UMemLazy
 import Xv6.ProofUvmcreate
 import Xv6.LinkUvmcreate
 import Xv6.UPtWalkaddrLemmas
